# Pythagorean Identities

1. **Complete the statement of the following Theorem.**

**Theorem 1 (Pythagorean Theorem)**

For any right triangle, if $c$ is the length of the hypotenuse and if $a$ and $b$ are the lengths of the remaining two sides, then the following equation holds:

$$a^2+b^2=c^2$$

2. **Draw a right triangle with hypotenuse of length 1. Label one of the non-square angles $\theta$. Label the side opposite to $\theta$ with $\sin\theta$. Label the side adjacent to $\theta$ with $\cos\theta$.**

![](https://cdn.jsdelivr.net/gh/FgSurewin/pictures/img/图片1.jpg)

**Use the Pythagorean Theorem to show that $\displaystyle{\sin^2\theta+\cos^2\theta=1}$.**

Given the Theorem 1, we have

$$a^2+b^2=c^2$$

So , we got

$$\sin^2(\theta)+\cos^2(\theta)=1$$

3. **Define $\displaystyle{\tan\theta=\frac{\sin\theta}{\cos\theta}}$ and $\displaystyle{\sec\theta=\frac{1}{\cos\theta}}$. Use the Pythagorean Theorem to show that $\displaystyle{\sec^2\theta=\tan^2\theta+1}$.**

We need to prove

$$\sec^2\theta- \tan^2\theta=1$$

Given the condition, we have

$$\sec^2\theta- \tan^2\theta=\frac{1}{\cos^2(\theta)}-\frac{\sin^2(\theta)}{\cos^2(\theta)}=\frac{1-\sin^2(\theta)}{\cos^2(\theta)}$$

Use Theorem 1

$$\sec^2\theta- \tan^2\theta=\frac{\cos^2(\theta)}{\cos^2(\theta)}=1$$

END.
